README.md
@@ -1,3 +1,5 @@
 # Simply Typed Lambda Calculus Formalization
 
 [stlc.v](stlc.v)
+
+Create Makefile with `coq_makefile -f _CoqProject *.v -o Makefile`
